exercise5.v
@@ -1,0 +1,256 @@
+From mathcomp Require Import mini_ssreflect.
+
+Set Implicit Arguments.
+Unset Strict Implicit.
+Unset Printing Implicit Defensive.
+(**
+----------------------------------------------------------
+#<div class="slide">#
+
+** Exercise 1:
+
+- Improve the last symplification function of lesson 5 by adding
+  the simplification rule #$$x - 0 = x$$#
+
+#<div>#
+*)
+
+Module Ex1.
+
+Inductive expr :=
+  | Zero
+  | Minus (x : expr) (y : expr)
+  | Var (n : nat).
+
+Fixpoint simplify e :=
+  match e with
+  | Minus x y =>
+      match simplify x, simplify y with
+      | Var n, Var m =>
+          match n == m with
+          | true => Zero
+          | false => Minus (Var n) (Var m)
+          end
+      | (* Fill me *)
+(*D*)    a, Zero => a
+      | a, b => Minus a b
+      end
+  | y => y
+  end.
+
+Fixpoint interp (e : expr) (c : list nat) :=
+  match e with
+  | Zero => 0
+  | Minus x y => (interp x c) - (interp y c)
+  | Var x => nth 0 c x
+  end.
+
+Lemma simplify_correct (e : expr) (c : list nat) : interp e c = interp (simplify e) c.
+Proof.
+elim: e => //= x Hx y Hy.
+case: (simplify x) Hx => [|x1 x2|n] -> ; case: (simplify y) Hy => [|y1 y2|m] -> //.
+(* fill in *)
+(*D*)1,2: by rewrite subn0.
+by case: eqP => [->|//]; rewrite subnn.
+Qed.
+
+
+Lemma test (x : nat) : x - x - 0 = 0.
+Proof.
+pose AST : expr := Minus (Minus (Var 0) (Var 0)) Zero.
+pose CTX : list nat := [:: x].
+rewrite -[LHS]/(interp AST CTX).
+rewrite simplify_correct.
+rewrite /=.
+by [].
+Qed.
+
+End Ex1.
+(**
+#</div>#
+
+----------------------------------------------------------
+#<div class="slide">#
+
+** Exercise 2:
+
+- Improve on exercise 1 by adding
+  to the [expr] data type a node for multiplication and
+  the simplification rules #$$x * 0 = 0$$# and #$$0 * x = 0$$#
+
+#<div>#
+*)
+Module Ex2.
+
+Inductive expr :=
+  | Zero
+  | (* fill in *)
+(*D*) Mult (x : expr) (y : expr)
+  | Minus (x : expr) (y : expr)
+  | Var (n : nat).
+
+Fixpoint simplify e :=
+  match e with
+  | Minus x y =>
+      match simplify x, simplify y with
+      | Var n, Var m =>
+          match n == m with
+          | true => Zero
+          | false => Minus (Var n) (Var m)
+          end
+      | (* Fill me, from ex 1*)
+(*D*)    a, Zero => a
+      | a, b => Minus a b
+      end
+  | (* fill me *)
+(*D*) Mult x y =>
+(*D*)       match simplify x, simplify y with
+(*D*)       | Zero, _ => Zero
+(*D*)       | _, Zero => Zero
+(*D*)       | a, b => Mult a b
+(*D*)       end
+  | y => y
+  end.
+
+Fixpoint interp (e : expr) (c : list nat) :=
+  match e with
+  | Zero => 0
+  | Minus x y => (interp x c) - (interp y c)
+  | (* fill in *)
+(*D*) Mult x y => (interp x c) * (interp y c)
+  | Var x => nth 0 c x
+  end.
+
+Lemma simplify_correct (e : expr) (c : list nat) : interp e c = interp (simplify e) c.
+Proof.
+elim: e => //= x Hx y Hy.
+- case: (simplify x) Hx => [|x1 x2|x1 x2|n] -> ; case: (simplify y) Hy => [|y1 y2|y1 y2|m] -> //.
+  (* fill in *)
+(*D*) 1,2,3: by rewrite muln0.
+- case: (simplify x) Hx => [|x1 x2|x1 x2|n] -> ; case: (simplify y) Hy => [|y1 y2|y1 y2|m] -> //.
+  (* fill in, like in exercise 1 *)
+(*D*) 1,2,3: by rewrite subn0.
+  by case: eqP => [->|//]; rewrite subnn.
+Qed.
+
+Lemma test (x : nat) (y : nat) : x - x - (y * 0) = 0.
+Proof.
+pose AST : expr := (* fill me *)
+(*D*)Minus (Minus (Var 0) (Var 0)) (Mult (Var 1) Zero).
+pose CTX : list nat := (* fill me *)
+(*D*)[:: x; y].
+rewrite -[LHS]/(interp AST CTX).
+rewrite simplify_correct.
+rewrite /=.
+by [].
+Qed.
+
+End Ex2.
+
+(**
+#</div>#
+
+----------------------------------------------------------
+#<div class="slide">#
+
+** Exercise 3:
+
+- Improve on exercise 2 by adding
+  to the [expr] data type a node for One and
+  the simplification rules #$$x * 1 = x$$# and #$$1 * x = x$$#
+
+#<div>#
+*)
+Module Ex3.
+
+Inductive expr :=
+  | Zero
+  | (* fill in *)
+(*D*) One
+  | (* fill in, as in exercise 2 *)
+(*D*) Mult (x : expr) (y : expr)
+  | Minus (x : expr) (y : expr)
+  | Var (n : nat).
+
+Fixpoint simplify e :=
+  match e with
+  | Minus x y =>
+      match simplify x, simplify y with
+      | Var n, Var m =>
+          match n == m with
+          | true => Zero
+          | false => Minus (Var n) (Var m)
+          end
+      | (* Fill me, from ex 1*)
+(*D*)    a, Zero => a
+      | a, b => Minus a b
+      end
+  | (* fill me *)
+(*D*) Mult x y =>
+(*D*)       match simplify x, simplify y with
+(*D*)       | Zero, _ => Zero
+(*D*)       | _, Zero => Zero
+(*D*)       | One, b => b
+(*D*)       | a, One => a
+(*D*)       | a, b => Mult a b
+(*D*)       end
+  | y => y
+  end.
+
+Fixpoint interp (e : expr) (c : list nat) :=
+  match e with
+  | Zero => 0
+  | (* fill in *)
+(*D*) One => 1
+  | Minus x y => (interp x c) - (interp y c)
+  | (* fill in *)
+(*D*) Mult x y => (interp x c) * (interp y c)
+  | Var x => nth 0 c x
+  end.
+
+Lemma simplify_correct (e : expr) (c : list nat) : interp e c = interp (simplify e) c.
+Proof.
+elim: e => //= x Hx y Hy.
+- case: (simplify x) Hx => [||x1 x2|x1 x2|n] -> ; case: (simplify y) Hy => [||y1 y2|y1 y2|m] -> //.
+  (* fill in *)
+(*D*) 1,2,3: by rewrite mul1n.
+(*D*) 1,3,5: by rewrite muln0.
+(*D*) 1,2,3: by rewrite muln1.
+- case: (simplify x) Hx => [||x1 x2|x1 x2|n] -> ; case: (simplify y) Hy => [||y1 y2|y1 y2|m] -> //.
+  (* fill in *)
+(*D*) 1,2,3: by rewrite subn0.
+(*D*) by case: eqP => [->|//]; rewrite subnn.
+Qed.
+
+Lemma test (x : nat) (y : nat) : x - x - (y * 0) = 0.
+Proof.
+pose AST : expr := (* fill me *)
+(*D*)Minus (Minus (Var 0) (Var 0)) (Mult (Var 1) Zero).
+pose CTX : list nat := (* fill me *)
+(*D*)[:: x; y].
+rewrite -[LHS]/(interp AST CTX).
+rewrite simplify_correct.
+rewrite /=.
+by [].
+Qed.
+
+End Ex3.
+
+
+
+(*
+#</div>#
+
+- computation is powerful on closed terms
+- proof size is constant
+
+
+#</div>#
+----------------------------------------------------------
+#<div class="slide vfill">#
+
+** To sum up
+
+#</div>#
+----------------------------------------------------------
+*)
